theories/prelude/base.v
@@ -1,4 +1,4 @@
-From iris.algebra Require Export base.
+From iris.prelude Require Export prelude.
 From iris.base_logic Require Import upred.
 From iris.program_logic Require Import weakestpre.
 From iris.base_logic Require Import invariants.
